erasure/theories/EEtaExpandedFix.v
@@ -9,7 +9,7 @@ From MetaCoq.PCUIC Require Import PCUICAst PCUICAstUtils
      PCUICValidity PCUICPrincipality PCUICElimination PCUICSN.
 
 From MetaCoq.Template Require Import config utils BasicAst Universes.
-From MetaCoq.Erasure Require Import EAst EGlobalEnv EAstUtils EEnvMap EExtends.
+From MetaCoq.Erasure Require Import EAst EGlobalEnv EAstUtils EEnvMap EExtends EWellformed.
 From MetaCoq.Erasure Require Import EWcbvEval EWcbvEvalInd.
 
 Set Default Proof Using "Type*".
@@ -73,7 +73,7 @@ Inductive expanded (Γ : list nat): term -> Prop :=
     expanded Γ (tCase (ind, pars) discr branches)
 | expanded_tProj (proj : projection) (t : term) : expanded Γ t -> expanded Γ (tProj proj t)
 | expanded_tFix (mfix : mfixpoint term) (idx : nat) args d : 
-  Forall (fun d => 
+  Forall (fun d => isLambda d.(dbody) /\
            let ctx := rev_map (fun  d => 1 + d.(rarg)) mfix in
           expanded (ctx ++ Γ) d.(dbody)) mfix ->
   Forall (expanded Γ) args ->
@@ -135,6 +135,7 @@ Lemma expanded_ind :
          (d : def term),
           Forall
             (λ d0 : def term,
+                isLambda d0.(dbody) /\
                 let ctx := rev_map (fun  d => 1 + d.(rarg)) mfix in
                 expanded Σ (ctx ++ Γ) (dbody d0)) mfix
           → Forall
@@ -178,14 +179,13 @@ Proof.
   - assert (Forall (P Γ) args). { clear - H0 f. induction H0; econstructor; eauto. }
     eapply HFix; eauto.
     revert H. clear - f.
-    generalize mfix at 1 3. intros mfix0 H.  induction H; econstructor; cbn in *; eauto; split.
+    generalize mfix at 1 3. intros mfix0 H. induction H; econstructor; cbn in *; intuition eauto; split.
   - eapply HCoFix; eauto.
     revert H. clear - f.
     generalize mfix at 1 3. intros mfix0 H.  induction H; econstructor; cbn in *; eauto; split.
   - eapply HConstruct; eauto.
     clear - H1 f. induction H1; econstructor; eauto.
 Qed.
-
 
 Definition expanded_constant_decl Σ (cb : constant_body) : Prop :=
   on_Some_or_None (expanded Σ []) cb.(cst_body).
@@ -304,8 +304,9 @@ Section isEtaExp.
     | tLambda na M => isEtaExp (0 :: Γ) M
     | tApp u v napp nnil with expanded_head_viewc u := 
       { | expanded_head_construct ind i => isEtaExp_app ind i (List.length v) && forallb_InP v (fun x H => isEtaExp Γ x)
-        | expanded_head_fix mfix idx => isEtaExp_fixapp mfix idx (List.length v) && 
-                                        forallb_InP mfix (fun x H => isEtaExp (rev_map (S ∘ rarg) mfix ++ Γ) x.(dbody)) && forallb_InP v (fun x H => isEtaExp Γ x)
+        | expanded_head_fix mfix idx => 
+          isEtaExp_fixapp mfix idx (List.length v) && 
+          forallb_InP mfix (fun x H => isLambda x.(dbody) && isEtaExp (rev_map (S ∘ rarg) mfix ++ Γ) x.(dbody)) && forallb_InP v (fun x H => isEtaExp Γ x)
         | expanded_head_rel n => option_default (fun m => m <=? List.length v) (nth_error Γ n) false && forallb_InP v (fun x H => isEtaExp Γ x) 
         | expanded_head_other _ _ => isEtaExp Γ u && forallb_InP v (fun x H => isEtaExp Γ x) }
     | tLetIn na b b' => isEtaExp Γ b && isEtaExp (0 :: Γ) b'
@@ -355,7 +356,8 @@ Section isEtaExp.
     ~~ isApp f -> v <> [] ->
     isEtaExp Γ (mkApps f v) = match expanded_head_viewc f with 
       | expanded_head_construct ind i => isEtaExp_app ind i #|v| && forallb (isEtaExp Γ) v
-      | expanded_head_fix mfix idx => isEtaExp_fixapp mfix idx #|v| && forallb (fun x => isEtaExp (rev_map (S ∘ rarg) mfix ++ Γ) x.(dbody)) mfix && forallb (isEtaExp Γ) v
+      | expanded_head_fix mfix idx => isEtaExp_fixapp mfix idx #|v| && 
+        forallb (fun x => isLambda x.(dbody) && isEtaExp (rev_map (S ∘ rarg) mfix ++ Γ) x.(dbody)) mfix && forallb (isEtaExp Γ) v
       | expanded_head_rel n => option_default (fun m => m <=? List.length v) (nth_error Γ n) false && forallb (fun x => isEtaExp Γ x) v
       | expanded_head_other t discr => isEtaExp Γ f && forallb (isEtaExp Γ) v
     end.
@@ -363,7 +365,7 @@ Section isEtaExp.
     rewrite isEtaExp_equation_1.
     intros napp hv.
     destruct (TermSpineView.view_mkApps (TermSpineView.view (mkApps f v)) napp hv) as [hna [hv' ->]].
-    cbn. destruct (expanded_head_viewc f); cbn; simp isEtaExp => //.
+    cbn -[isEtaExp]. destruct (expanded_head_viewc f); cbn -[isEtaExp]; simp isEtaExp => //.
   Qed.
 
   Tactic Notation "simp_eta" "in" hyp(H) := simp isEtaExp in H; rewrite -?isEtaExp_equation_1 in H.
@@ -374,7 +376,9 @@ Section isEtaExp.
   Lemma isEtaExp_mkApps Γ f v : ~~ isApp f -> 
     isEtaExp Γ (mkApps f v) = match expanded_head_viewc f with 
       | expanded_head_construct ind i => isEtaExp_app ind i #|v| && forallb (isEtaExp Γ) v
-      | expanded_head_fix mfix idx => isEtaExp_fixapp mfix idx #|v| && forallb (fun x => isEtaExp (rev_map (S ∘ rarg) mfix ++ Γ) x.(dbody)) mfix && forallb (isEtaExp Γ) v
+      | expanded_head_fix mfix idx => 
+        isEtaExp_fixapp mfix idx #|v| && 
+        forallb (fun x => isLambda x.(dbody) && isEtaExp (rev_map (S ∘ rarg) mfix ++ Γ) x.(dbody)) mfix && forallb (isEtaExp Γ) v
       | expanded_head_rel n => option_default (fun m => m <=? List.length v) (nth_error Γ n) false && forallb (fun x => isEtaExp Γ x) v
       | expanded_head_other t discr => isEtaExp Γ f && forallb (isEtaExp Γ) v
     end.
@@ -459,7 +463,7 @@ Section isEtaExp.
     - rewrite app_assoc. eapply a, b. reflexivity.
     - rewrite isEtaExp_mkApps => //. cbn [expanded_head_viewc]. rtoProp; repeat solve_all.
     - rewrite isEtaExp_mkApps => //. cbn [expanded_head_viewc]. rtoProp; repeat solve_all.
-      rewrite app_assoc. eapply a, b. reflexivity.
+      rewrite app_assoc. rtoProp; intuition auto.
     - rewrite isEtaExp_mkApps => //. cbn [expanded_head_viewc]. rtoProp; repeat solve_all.
       destruct nth_error eqn:E; try easy. erewrite nth_error_app_Some; eauto.
     - rewrite isEtaExp_mkApps => //. rewrite Heq. rtoProp; repeat solve_all.
@@ -480,7 +484,7 @@ Section isEtaExp.
       eapply nth_error_Some_length in Hn. now eapply Nat.ltb_lt.
     - eapply a in b. 2: f_equal. revert b. now len.
     - eapply a in b. 2: f_equal. revert b. now len.
-    - cbn. solve_all. eapply a in b. 2: reflexivity. revert b. now len.
+    - cbn. solve_all. rtoProp; intuition auto. eapply a in H0. 2: reflexivity. revert H0. now len.
     - destruct nth_error eqn:Hn; cbn in H1; try easy.
       eapply nth_error_Some_length in Hn. now eapply Nat.ltb_lt.
   Qed.
@@ -520,7 +524,8 @@ Section isEtaExp.
       rtoProp; repeat split.
       + rewrite /isEtaExp_fixapp in eu |- *. rewrite nth_error_map. destruct nth_error; try congruence.
         cbn. now len.
-      + solve_all.
+      + solve_all. rtoProp; intuition auto.
+        now eapply isLambda_csubst.
         rewrite app_assoc.  eapply a0; len; eauto. cbn. f_equal.
         rewrite app_assoc. do 2 f_equal.
         rewrite !rev_map_spec. f_equal. rewrite map_map. now eapply map_ext.      
@@ -552,25 +557,28 @@ Section isEtaExp.
     #|Γ| = k ->
     nth_error mfix idx = Some d ->
     closed (EAst.tFix mfix idx) ->
-    forallb (fun x => isEtaExp (rev_map (S ∘ rarg) mfix) x.(dbody)) mfix ->
+    forallb (fun x => isLambda x.(dbody) &&  isEtaExp (rev_map (S ∘ rarg) mfix) x.(dbody)) mfix ->
     isEtaExp (Γ ++ [1 + d.(EAst.rarg)] ++ Δ) b -> isEtaExp (Γ ++ Δ) (ECSubst.csubst (EAst.tFix mfix idx) k b).
   Proof using Type*.
     intros Hk Hnth Hcl. 
     remember (Γ ++ [1 + d.(EAst.rarg)] ++ Δ)%list as Γ_.
     funelim (isEtaExp Γ_ b); try simp_eta; eauto; try fold csubst;
-      try toAll; try now repeat solve_all; subst.
+      try toAll; try solve_all; subst.
     - intros. simp isEtaExp ; cbn. destruct (Nat.compare_spec #|Γ0| i) => //; simp_eta.
       + rewrite nth_error_app2 in H0; try lia; cbn in H0; try easy. subst. rewrite minus_diag in H0. cbn in H0. easy.
       + rewrite !nth_error_app2 in H0 |- *; cbn; try lia.
         erewrite option_default_ext; eauto. f_equal.
         destruct i; cbn; lia.
       + now rewrite !nth_error_app1 in H0 |- *; try lia.
-    - intros. solve_all. eapply a; eauto. solve_all.
+    - intros. eapply forallb_All in H1; eapply All_mix in H; tea.
+      eapply All_forallb, All_map, All_impl; tea; cbv beta.
+      intros x Hx. eapply Hx; eauto. apply Hx.
     - eapply H with (Γ := 0 :: Γ0); cbn -[isEtaExp]; eauto. 
     - solve_all. move/andP: H2 => [] etab etab'. simp_eta.
       apply/andP. split; eauto.
-      eapply H0 with (Γ := 0 :: Γ0); cbn; eauto.
-    - solve_all. rtoProp. intuition eauto.
+      eapply H; eauto. solve_all.
+      eapply H0 with (Γ := 0 :: Γ0); eauto. solve_all.
+    - rtoProp. intuition eauto.
       solve_all. rewrite app_assoc. eapply a; cbn-[isEtaExp]; eauto. now len. cbn.
       now rewrite app_assoc.
       solve_all.
@@ -582,9 +590,12 @@ Section isEtaExp.
       rewrite csubst_mkApps /=.
       rewrite isEtaExp_Constructor. solve_all.
       rewrite map_length. rtoProp; solve_all.
-      solve_all.
-      eapply a; eauto.
-      solve_all.
+      rewrite forallb_map. 
+      eapply All_forallb. clear Heq0 Heq.
+      eapply All_impl; tea; cbv beta.
+      intros x Hx.
+      eapply Hx; eauto.
+      solve_all. apply Hx.
     - solve_all. rewrite csubst_mkApps /=.
       move/andP : H2 => [] /andP [] eu ef ev.
       rewrite isEtaExp_mkApps //.
@@ -593,38 +604,49 @@ Section isEtaExp.
       + rewrite /isEtaExp_fixapp in eu |- *. rewrite nth_error_map.
         destruct (nth_error mfix idx); try congruence.
         cbn. now len.
-      + solve_all.
+      + solve_all. rtoProp; intuition auto. now eapply isLambda_csubst.
         rewrite app_assoc.  eapply a; len; eauto.
         { cbn in Hcl. solve_all. rewrite Nat.add_0_r in a0. eauto. }
         cbn. f_equal.
         rewrite app_assoc. do 2 f_equal.
         rewrite !rev_map_spec. f_equal. rewrite map_map. now eapply map_ext.
         solve_all.      
-      + solve_all. eapply a; eauto. solve_all.
+      + eapply forallb_All in ev; eapply All_mix in H0; tea.
+        eapply All_forallb, All_map, All_impl; tea; cbv beta.
+        intros x Hx. eapply Hx; eauto. solve_all. apply Hx.
     - rewrite csubst_mkApps /=. rtoProp. destruct (Nat.compare_spec #|Γ0| n) => //; simp_eta.
       + rewrite isEtaExp_mkApps => //. cbn [expanded_head_viewc].
         rtoProp. repeat split; eauto.
-        * unfold isEtaExp_fixapp. rewrite Hnth. len. destruct H2 as [Hn H2].
-          subst. rewrite nth_error_app2 in Hn; try lia.
-          rewrite minus_diag in Hn. cbn in Hn. eapply Nat.ltb_lt.
-          eapply Nat.leb_le in Hn. lia.        
-        * cbn in Hcl. solve_all.
+        * unfold isEtaExp_fixapp. rewrite Hnth. len.
+          subst. rewrite nth_error_app2 in H1; try lia.
+          rewrite minus_diag in H1. cbn in H1. eapply Nat.ltb_lt.
+          eapply Nat.leb_le in H1. lia.        
+        * cbn in Hcl. solve_all. rtoProp; intuition auto.
           now eapply expanded_weakening.
-        * destruct H2. solve_all. eapply a ;eauto. solve_all.          
+        * eapply forallb_All in H2. eapply All_mix in H; tea.
+          eapply All_forallb, All_map, All_impl; tea; cbv beta.
+          intros x Hx. eapply Hx; eauto. apply Hx.
       + rewrite isEtaExp_mkApps; eauto. cbn [expanded_head_viewc].
-        rtoProp. intros. destruct H2. split. 2:{ solve_all. eapply a; eauto. solve_all. }
-        rewrite !nth_error_app2 in H2 |- *; try lia.
-        rewrite (nth_error_app2 ([S (EAst.rarg d)])) in H2; cbn; try lia.
-        len.
+        rtoProp. intros.
+        split. 2:{
+          eapply forallb_All in H2; eapply All_mix in H; tea; clear H2.      
+          eapply All_forallb, All_map, All_impl; tea; cbv beta.
+          intros x Hx. eapply Hx; eauto. apply Hx. }
+        rewrite !nth_error_app2 in H1 |- *; cbn; try lia. len.
         erewrite option_default_ext. eauto. f_equal.
         destruct n; cbn; lia.
       + rewrite isEtaExp_mkApps; eauto. cbn [expanded_head_viewc].
-        intros. destruct H2.
-        rtoProp. split. 2:{ solve_all. eapply a; eauto. solve_all. }
+        intros. rtoProp. split. 2:{
+          eapply forallb_All in H2; eapply All_mix in H; tea; clear H2.      
+          eapply All_forallb, All_map, All_impl; tea; cbv beta.
+          intros x Hx. eapply Hx; eauto. apply Hx. }
         len.
-        now rewrite !nth_error_app1 in H2 |- *; try lia.
+        now rewrite !nth_error_app1 in H1 |- *; try lia.
     - intros. rtoProp. rewrite csubst_mkApps /=.
-      eapply isEtaExp_mkApps_intro => //. 2:{ solve_all. eapply a; eauto. solve_all. }
+      eapply isEtaExp_mkApps_intro => //.
+       2:{ eapply forallb_All in H3; eapply All_mix in H0; tea; clear H3.      
+        eapply All_map, All_impl; tea; cbv beta.
+        intros x Hx. eapply Hx; eauto. apply Hx. }
       eapply H; eauto.
   Qed.
   
@@ -641,12 +663,13 @@ Section isEtaExp.
   Qed.
 
   Lemma isEtaExp_fixsubstl Δ mfix t : 
-    forallb (fun x => isEtaExp (rev_map (S ∘ rarg) mfix) x.(dbody)) mfix ->
+    forallb (fun x => isLambda x.(dbody) &&
+      isEtaExp (rev_map (S ∘ rarg) mfix) x.(dbody)) mfix ->
     isEtaExp ((rev_map (S ∘ rarg) mfix) ++ Δ) t ->
     isEtaExp Δ (substl (fix_subst mfix) t).
   Proof using Type*.
     intros Hall Heta.
-    assert (Hcl : closed (EAst.tFix mfix 0) ). { cbn. solve_all. eapply isEtaExp_closed in H. revert H. now len. }
+    assert (Hcl : closed (EAst.tFix mfix 0) ). { cbn. solve_all. rtoProp; intuition auto. eapply isEtaExp_closed in H0. revert H0. now len. }
     revert Hcl Hall Heta.  
     intros Hcl Hall Heta.
     cbn in Hcl. solve_all.
@@ -718,26 +741,27 @@ Section isEtaExp.
   Qed. 
   
   Lemma isEtaExp_cunfold_fix mfix idx n f : 
-    forallb (isEtaExp (rev_map (S ∘ rarg) mfix) ∘ dbody) mfix ->
-    Ee.cunfold_fix mfix idx = Some (n, f) ->
+    forallb (fun d => isLambda d.(dbody) && isEtaExp (rev_map (S ∘ rarg) mfix) d.(dbody)) mfix ->
+    EGlobalEnv.cunfold_fix mfix idx = Some (n, f) ->
     isEtaExp [] f.
   Proof.
     intros heta.
-    unfold Ee.cunfold_fix.
+    unfold EGlobalEnv.cunfold_fix.
     destruct nth_error eqn:heq => //.
     intros [= <- <-] => /=.
     eapply isEtaExp_fixsubstl.
-    - solve_all.
+    - solve_all; rtoProp; intuition auto.
     - rewrite app_nil_r. solve_all. eapply All_nth_error in heta; eauto.
+      now move/andP: heta.
   Qed.
   
   Lemma isEtaExp_cunfold_cofix mfix idx n f : 
     forallb (isEtaExp (repeat 0 #|mfix|) ∘ dbody) mfix ->
-    Ee.cunfold_cofix mfix idx = Some (n, f) ->
+    EGlobalEnv.cunfold_cofix mfix idx = Some (n, f) ->
     isEtaExp [] f.
   Proof.
     intros heta.
-    unfold Ee.cunfold_cofix.
+    unfold EGlobalEnv.cunfold_cofix.
     destruct nth_error eqn:heq => //.
     intros [= <- <-] => /=.
     eapply isEtaExp_substl.
@@ -751,7 +775,8 @@ Section isEtaExp.
     let (hd, v) := decompose_app (mkApps f u) in
     match expanded_head_viewc hd with
       | expanded_head_construct ind i => isEtaExp_app ind i #|v| && forallb (isEtaExp Γ) v
-      | expanded_head_fix mfix idx => isEtaExp_fixapp mfix idx #|v| && forallb (fun x => isEtaExp (rev_map (S ∘ rarg) mfix ++ Γ) x.(dbody)) mfix && forallb (isEtaExp Γ) v
+      | expanded_head_fix mfix idx => isEtaExp_fixapp mfix idx #|v| && 
+        forallb (fun x => isLambda x.(dbody) && isEtaExp (rev_map (S ∘ rarg) mfix ++ Γ) x.(dbody)) mfix && forallb (isEtaExp Γ) v
       | expanded_head_rel n => (option_default (fun m => m <=? List.length v) (nth_error Γ n) false) && forallb (fun x => isEtaExp Γ x) v
       | expanded_head_other t discr => isEtaExp Γ hd && forallb (isEtaExp Γ) v
       end. (* 
@@ -781,13 +806,14 @@ Lemma isEtaExp_app_expanded Σ ind idx n :
 Proof.
   unfold isEtaExp_app, lookup_constructor_pars_args, lookup_inductive, lookup_minductive.
   split.
-  - intros H.
+  - intros H. cbn in H.
     destruct lookup_env as [[| mind] | ] eqn:E; cbn in H; try congruence.
     destruct nth_error as [ idecl | ] eqn:E2; cbn in H; try congruence.
     destruct (nth_error (E.ind_ctors idecl) idx) as [ [cname ?] | ] eqn:E3; cbn in H; try congruence.
     repeat esplit.
     red. all: eauto. eapply leb_iff in H. lia.
   - intros (? & ? & ? & ? & [[]] & Hle).
+    cbn.
     rewrite H. cbn. rewrite H0. cbn. rewrite H1. cbn.
     eapply leb_iff. eauto.
 Qed.
@@ -820,7 +846,7 @@ Proof.
   - rtoProp. rewrite forallb_InP_spec in H2. rewrite forallb_InP_spec in H3. eapply In_All in H. eapply In_All in H0. 
     unfold isEtaExp_fixapp in H1. destruct nth_error eqn:E; try congruence.
     eapply expanded_tFix.
-    all: try now solve_all.
+    all: try now solve_all. solve_all; rtoProp; intuition auto.
     eapply Nat.ltb_lt in H1. lia.
   - rtoProp. destruct (nth_error) eqn:Hn; invs H0.
     econstructor. eauto. eapply Nat.leb_le; eauto.  rewrite forallb_InP_spec in H1.
@@ -846,7 +872,7 @@ Proof.
   - eapply isEtaExp_mkApps_intro; eauto. solve_all. 
   - rewrite isEtaExp_mkApps //. cbn [expanded_head_viewc]. rtoProp. repeat split.
     + unfold isEtaExp_fixapp. rewrite H4. eapply Nat.ltb_lt. lia.
-    + solve_all.
+    + solve_all; rtoProp; intuition auto.
     + solve_all.
   - rewrite isEtaExp_Constructor. eapply andb_true_iff.
     split. 2: eapply forallb_Forall.
@@ -880,7 +906,7 @@ Lemma lookup_inductive_pars_constructor_pars_args Σ {ind n pars args} :
   lookup_inductive_pars Σ (inductive_mind ind) = Some pars.
 Proof.
   rewrite /lookup_constructor_pars_args /lookup_inductive_pars.
-  rewrite /lookup_inductive. destruct lookup_minductive => //.
+  unfold lookup_constructor, lookup_inductive. destruct lookup_minductive => //.
   cbn. do 2 destruct nth_error => //. congruence.
 Qed.
 
@@ -894,7 +920,7 @@ Lemma isEtaExp_tApp' {Σ} {Γ} {f u} : isEtaExp Σ Γ (tApp f u) ->
     isEtaExp_app Σ kn c #|args| && forallb (isEtaExp Σ Γ) args
   | expanded_head_fix mfix idx => 
     args <> [] /\ f = mkApps hd (remove_last args) /\ u = last args u /\ 
-    isEtaExp_fixapp mfix idx #|args| && forallb (fun d => isEtaExp Σ (rev_map (fun  d => 1 + d.(rarg)) mfix ++ Γ) d.(dbody)) mfix && forallb (isEtaExp Σ Γ) args
+    isEtaExp_fixapp mfix idx #|args| && forallb (fun d => isLambda d.(dbody) && isEtaExp Σ (rev_map (fun  d => 1 + d.(rarg)) mfix ++ Γ) d.(dbody)) mfix && forallb (isEtaExp Σ Γ) args
   | expanded_head_rel n => 
     args <> [] /\ f = mkApps hd (remove_last args) /\ u = last args u /\ 
     option_default (fun m => m <=? List.length args) (nth_error Γ n) false && forallb (fun x => isEtaExp Σ Γ x) args
@@ -965,20 +991,20 @@ Proof.
       now exists ((kn', d')::Σ'').
 Qed.
 
-Lemma isEtaExp_app_extends Σ Σ' ind k n :
+Lemma isEtaExp_app_extends {efl : EEnvFlags} Σ Σ' ind k n :
   extends Σ Σ' ->
   wf_glob Σ' -> 
   isEtaExp_app Σ ind k n ->
   isEtaExp_app Σ' ind k n.
 Proof.
   rewrite /isEtaExp_app.
-  rewrite /lookup_constructor_pars_args /lookup_inductive /lookup_minductive.
+  rewrite /lookup_constructor_pars_args /lookup_constructor /lookup_inductive /lookup_minductive.
   move=> ext wf.
   destruct (lookup_env Σ _) eqn:hl => //.
   rewrite (extends_lookup wf ext hl) /= //.
 Qed.
 
-Lemma isEtaExp_extends Σ Σ' Γ t : 
+Lemma isEtaExp_extends {efl : EEnvFlags} Σ Σ' Γ t : 
   extends Σ Σ' ->
   wf_glob Σ' ->
   isEtaExp Σ Γ t ->
@@ -996,14 +1022,14 @@ Proof.
     solve_all.
   - eapply In_All in H, H0. rewrite isEtaExp_mkApps => //.
     cbn [expanded_head_viewc]. rtoProp. repeat split; eauto.
-    all: solve_all.
+    all: solve_all; rtoProp; intuition eauto.
   - eapply In_All in H. rewrite isEtaExp_mkApps => //.
     cbn [expanded_head_viewc]. rtoProp. repeat split; eauto.
     all: solve_all.
   - eapply In_All in H0. apply isEtaExp_mkApps_intro; eauto. solve_all.
 Qed.
 
-Lemma isEtaExp_extends_decl Σ Σ' t : 
+Lemma isEtaExp_extends_decl {efl : EEnvFlags} Σ Σ' t : 
   extends Σ Σ' ->
   wf_glob Σ' ->
   isEtaExp_decl Σ t ->
@@ -1014,7 +1040,7 @@ Proof.
   now eapply isEtaExp_extends.
 Qed.
 
-Lemma isEtaExp_lookup {Σ kn d}: 
+Lemma isEtaExp_lookup {efl : EEnvFlags} {Σ kn d}: 
   isEtaExp_env Σ -> wf_glob Σ ->
   lookup_env Σ kn = Some d ->
   isEtaExp_decl Σ d.
@@ -1040,7 +1066,7 @@ Proof.
   intros. now eapply All_firstn.
 Qed.
 
-Lemma eval_etaexp {fl : Ee.WcbvFlags} {Σ a a'} : 
+Lemma eval_etaexp {fl : Ee.WcbvFlags} {efl : EEnvFlags} {Σ a a'} : 
   isEtaExp_env Σ ->
   wf_glob Σ ->
   Ee.eval Σ a a' -> isEtaExp Σ [] a -> isEtaExp Σ [] a'.
@@ -1394,7 +1420,7 @@ Proof.
     * destruct p; solve_discr. noconf H3.
       right. len.
       move: e; unfold isEtaExp_fixapp.
-      unfold Ee.cunfold_fix. destruct nth_error eqn:hnth => //.
+      unfold EGlobalEnv.cunfold_fix. destruct nth_error eqn:hnth => //.
       intros [=]. rewrite H3. rewrite -(All2_length a0). eapply Nat.ltb_lt; lia.
     * right. len. eapply isEtaExp_fixapp_mon; tea. lia.
   + eapply mkApps_eq in H1 as [? []] => //; subst.
@@ -1427,7 +1453,7 @@ Qed.
 
 Lemma isEtaExp_FixApp {Σ mfix idx l} :
   isEtaExp_fixapp mfix idx #|l| ->
-  forallb (λ d : def EAst.term, isEtaExp Σ (rev_map (λ d0 : def term, 1 + rarg d0) mfix ++ []) (dbody d)) mfix ->
+  forallb (λ d : def EAst.term, isLambda d.(dbody) && isEtaExp Σ (rev_map (λ d0 : def term, 1 + rarg d0) mfix ++ []) (dbody d)) mfix ->
   forallb (isEtaExp Σ []) l ->
   isEtaExp Σ [] (mkApps (tFix mfix idx) l).
 Proof.
@@ -1463,7 +1489,7 @@ Proof.
   now simp_eta in he.
 Qed.
 
-Lemma neval_to_stuck_fix {Σ mfix idx t} :
+Lemma neval_to_stuck_fix {efl : EEnvFlags} {Σ mfix idx t} :
   isEtaExp_env Σ ->
   wf_glob Σ ->
   isEtaExp Σ [] t -> @eval opt_wcbv_flags Σ t (tFix mfix idx) -> False.
@@ -1473,7 +1499,7 @@ Proof.
   now apply isEtaExp_tFix in H.
 Qed.
 
-Lemma neval_to_stuck_fix_app {fl Σ mfix idx t args} :
+Lemma neval_to_stuck_fix_app {efl : EEnvFlags} {fl Σ mfix idx t args} :
   with_guarded_fix ->
   isEtaExp_env Σ ->
   wf_glob Σ ->
@@ -1505,7 +1531,7 @@ Lemma isEtaExp_tApp_eval {fl} {Σ} {f u v} :
   | expanded_head_fix mfix idx =>
     args <> [] /\ f = mkApps hd (remove_last args) /\ u = last args u /\ 
     [&& isEtaExp_fixapp mfix idx #|remove_last args|,
-    forallb (fun d => isEtaExp Σ (rev_map (fun  d => 1 + d.(rarg)) mfix ++ []) d.(dbody)) mfix,
+    forallb (fun d => isLambda d.(dbody) && isEtaExp Σ (rev_map (fun  d => 1 + d.(rarg)) mfix ++ []) d.(dbody)) mfix,
     forallb (isEtaExp Σ []) (remove_last args) & isEtaExp Σ [] u]
   | expanded_head_rel n => False
   | expanded_head_other _ discr => 
@@ -1762,7 +1788,7 @@ Proof.
     eapply eval_app_cong_tApp'. now eapply eval_to_value in evf''. exact e0. exact evres.
 Qed.
 
-Lemma All_eval_etaexp {fl : WcbvFlags} Σ l l' :
+Lemma All_eval_etaexp {fl : WcbvFlags} {efl : EEnvFlags} Σ l l' :
   isEtaExp_env Σ ->
   wf_glob Σ ->
   All2 (eval Σ) l l' -> forallb (isEtaExp Σ []) l -> forallb (isEtaExp Σ []) l'.
@@ -1786,7 +1812,7 @@ Proof.
   intros h. now apply isFix_mkApps.
 Qed.
 
-Lemma eval_opt_to_target {fl: WcbvFlags} Σ t v :
+Lemma eval_opt_to_target {fl: WcbvFlags} {efl : EEnvFlags} Σ t v :
   with_guarded_fix ->
   isEtaExp_env Σ ->
   wf_glob Σ ->
@@ -2137,12 +2163,14 @@ Proof.
       eapply All_app in H2 as []. solve_all.
     * eapply erases_deps_mkApps_inv in etaΣ as [].
       depelim H7; simp_eta => //.
-      + eapply All2_nth_error_Some in H4; tea. destruct H4 as [? [? [? []]]]; tea.
+      + eapply All2_nth_error_Some in H4; tea. destruct H4 as [? [? []]]; tea.
         assert (rev_map (fun d1 : def term => S (rarg d1)) mfix = rev_map (fun d1 => S (EAst.rarg d1)) mfix').
-        { rewrite !rev_map_spec. f_equal. clear -X. induction X; cbn; auto. destruct r as [? []]. rewrite e0 IHX //. }
+        { rewrite !rev_map_spec. f_equal. clear -X. induction X; cbn; auto. destruct r as [eqb eqrar isl isl' e].
+          rewrite eqrar IHX //. }
         depelim H6.
         eapply EEtaExpandedFix.expanded_tFix; tea.
-        ++ cbn. rewrite -H6. solve_all.
+        ++ cbn. rewrite -H6. solve_all. apply b0.
+          eapply b1 => //. eapply b0.
         ++ solve_all.
         ++ intros hx0. subst x0. depelim H8 => //.
         ++ now rewrite -(Forall2_length H8) -e1.
