erasure/theories/ErasureFunction.v
@@ -519,11 +519,11 @@ Section Erase.
         E.tProj p c'
       | tFix mfix n :=
         let Γ' := (fix_context mfix ++ Γ)%list in
-        let mfix' := erase_mfix Γ' mfix _ in
+        let mfix' := erase_fix Γ' mfix _ in
         E.tFix mfix' n
       | tCoFix mfix n :=
         let Γ' := (fix_context mfix ++ Γ)%list in
-        let mfix' := erase_mfix Γ' mfix _ in
+        let mfix' := erase_cofix Γ' mfix _ in
         E.tCoFix mfix' n }
       (* erase Γ (tPrim p) Ht _ := E.tPrim (erase_prim p) *)
     } } 
@@ -545,14 +545,31 @@ Section Erase.
       let br' := erase (Γ ,,, inst_case_branch_context p br) (bbody br) _ in
       let brs' := erase_brs Γ p brs _ in
       (erase_context br.(bcontext), br') :: brs' }
-  where erase_mfix (Γ : context) (mfix : mfixpoint term)
+  
+  where erase_fix (Γ : context) (mfix : mfixpoint term)
     (Ht : forall Σ0 : global_env_ext, abstract_env_rel' Σ Σ0 ->
-          ∥ All (fun d => welltyped Σ0 Γ d.(dbody)) mfix ∥) : E.mfixpoint E.term :=
-  { erase_mfix Γ [] _ := [];
-    erase_mfix Γ (d :: mfix) Hmfix := 
+          ∥ All (fun d => isLambda d.(dbody) /\ welltyped Σ0 Γ d.(dbody)) mfix ∥) : E.mfixpoint E.term :=
+  { erase_fix Γ [] _ := [];
+    erase_fix Γ (d :: mfix) Hmfix := 
       let dbody' := erase Γ d.(dbody) _ in
+      let dbody' := if isBox dbody' then
+        match d.(dbody) with
+        (* We ensure that all fixpoint members start with a lambda, even a dummy one if the 
+           recursive definition is erased. *)
+        | tLambda na _ _ => E.tLambda (binder_name na) E.tBox
+        | _ => dbody'
+        end else dbody' in
       let d' := {| E.dname := d.(dname).(binder_name); E.rarg := d.(rarg); E.dbody := dbody' |} in
-      d' :: erase_mfix Γ mfix _ }
+      d' :: erase_fix Γ mfix _ }
+
+  where erase_cofix (Γ : context) (mfix : mfixpoint term)
+      (Ht : forall Σ0 : global_env_ext, abstract_env_rel' Σ Σ0 ->
+            ∥ All (fun d => welltyped Σ0 Γ d.(dbody)) mfix ∥) : E.mfixpoint E.term :=
+    { erase_cofix Γ [] _ := [];
+      erase_cofix Γ (d :: mfix) Hmfix := 
+        let dbody' := erase Γ d.(dbody) _ in
+        let d' := {| E.dname := d.(dname).(binder_name); E.rarg := d.(rarg); E.dbody := dbody' |} in
+        d' :: erase_cofix Γ mfix _ }
     .
   Proof. 
     all: try clear b'; try clear f';
@@ -590,13 +607,16 @@ Section Erase.
     - eapply inversion_Proj in Ht as (? & ? & ? & ? & ? & ? & ? & ? & ?); auto.
       eexists; eauto.
     - eapply inversion_Fix in Ht as (? & ? & ? & ? & ? & ?); auto.
-      sq. eapply All_impl; tea. cbn. intros d Ht; now eexists.
+      sq. destruct p. move/andP: i => [wffix _].
+      solve_all. now eexists.
     - eapply inversion_CoFix in Ht as (? & ? & ? & ? & ? & ?); auto.
       sq. eapply All_impl; tea. cbn. intros d Ht; now eexists.
     - sq. now depelim X.
     - sq. now depelim X.
     - sq. now depelim X.
     - sq. now depelim X.
+    - sq. now depelim X.
+    - clear dbody'0. specialize (Hmfix _ wfΣ'). sq. now depelim X.
     - sq. now depelim X.
     - sq. now depelim X.
   Qed.
@@ -622,20 +642,24 @@ Lemma erase_irrel (Σ : wf_env_ext) :
   (forall Γ t wt, forall wt', erase Σ Γ t wt = erase Σ Γ t wt') ×
   (forall Γ l wt, forall wt', erase_terms Σ Γ l wt = erase_terms Σ Γ l wt') ×
   (forall Γ p l wt, forall wt', erase_brs Σ Γ p l wt = erase_brs Σ Γ p l wt') ×
-  (forall Γ l wt, forall wt', erase_mfix Σ Γ l wt = erase_mfix Σ Γ l wt').
+  (forall Γ l wt, forall wt', erase_fix Σ Γ l wt = erase_fix Σ Γ l wt') ×
+  (forall Γ l wt, forall wt', erase_cofix Σ Γ l wt = erase_cofix Σ Γ l wt').
 Proof.
   apply: (erase_elim Σ
     (fun Γ t wt e => 
       forall wt' : forall Σ0 : global_env_ext, abstract_env_rel' Σ Σ0 ->  welltyped Σ0 Γ t, e = erase Σ Γ t wt')
     (fun Γ l awt e => forall wt', e = erase_terms Σ Γ l wt')
     (fun Γ p l awt e => forall wt', e = erase_brs Σ Γ p l wt')
-    (fun Γ l awt e => forall wt', e = erase_mfix Σ Γ l wt')); clear.
+    (fun Γ l awt e => forall wt', e = erase_fix Σ Γ l wt')
+    (fun Γ l awt e => forall wt', e = erase_cofix Σ Γ l wt')); clear.
   all:intros *; intros; simp_erase.
   all:try simp erase; try iserasableb_irrel; simp_erase => //.
   all:try clear he Heq.
   all:try bang.
   all:try solve [cbn; f_equal; eauto].
   all:try solve [cbn; repeat (f_equal; eauto)].
+  cbn. f_equal. f_equal. now rewrite (H (erase_obligation_19 Σ Γ d mfix wt')).
+  now rewrite (H0 (erase_obligation_20 Σ Γ d mfix wt')).
 Qed.
 
 Section map_All.
@@ -670,16 +694,6 @@ Proof.
   exists (tSort s). intuition auto. left; simpl; auto.
 Qed.
 
-Lemma is_box_mkApps f a : is_box (E.mkApps f a) = is_box f.
-Proof.
-  now rewrite /is_box EAstUtils.head_mkApps.
-Qed.
-
-Lemma is_box_tApp f a : is_box (E.tApp f a) = is_box f.
-Proof.
-  now rewrite /is_box EAstUtils.head_tApp.
-Qed.
-
 Lemma is_erasableb_reflect (Σ : wf_env_ext) Γ t wt : reflect (∥ isErasable Σ Γ t ∥) (is_erasableb Σ Γ t wt).
 Proof.
   unfold is_erasableb. destruct is_erasable; constructor => //.
@@ -698,6 +712,7 @@ Proof.
       if is_box e then ∥ isErasable Σ Γ t ∥ else ∥ isErasable Σ Γ t ∥ -> False)
     (fun Γ l awt e => True)
     (fun Γ p l awt e => True)
+    (fun Γ l awt e => True)
     (fun Γ l awt e => True)); intros.
 
   all:try discriminate; auto.
@@ -733,9 +748,15 @@ Proof.
                        (erase_context (bcontext x) = x'.1)) l e)
     (fun Γ l awt e => All2
     (fun (d : def term) (d' : E.def E.term) =>
-     (binder_name (dname d) = E.dname d') *
-     (rarg d = E.rarg d'
-      × Σ;;; Γ |- dbody d ⇝ℇ E.dbody d')) l e)); intros.
+     [× binder_name (dname d) = E.dname d',
+        rarg d = E.rarg d',
+        isLambda (dbody d), E.isLambda (E.dbody d') &
+        Σ;;; Γ |- dbody d ⇝ℇ E.dbody d']) l e)
+    (fun Γ l awt e => All2
+      (fun (d : def term) (d' : E.def E.term) =>
+        (binder_name (dname d) = E.dname d') *
+        (rarg d = E.rarg d'
+         × Σ;;; Γ |- dbody d ⇝ℇ E.dbody d')) l e)) ; intros.
     all:try discriminate.
     all:try bang.
     all:try match goal with 
@@ -746,24 +767,40 @@ Proof.
     all: try solve [constructor; eauto].
   all:try destruct Σ.(wf_env_ext_wf) as [wfΣ].
   all: cbn in *; assert (wfΣ' : abstract_env_rel' Σ Σ) by reflexivity;
-  pose proof (abstract_env_ext_wf _ wfΣ') as [wf];
+  try constructor; auto;
+  try pose proof (abstract_env_ext_wf _ wfΣ') as [wf];
   specialize_Σ wfΣ'.
   
-  - constructor. clear Heq.
+  - clear Heq.
     eapply nisErasable_Propositional in Ht; auto.
 
   - cbn.
-    constructor; auto. 
     destruct (Ht _ wfΣ').
     destruct (inversion_Case _ _ X0) as [mdecl [idecl []]]; eauto.
     eapply elim_restriction_works; eauto.
     intros isp. eapply isErasable_Proof in isp. eauto.
 
-  - constructor; auto. clear Heq.
+  - clear Heq.
     destruct (Ht _ wfΣ') as [? Ht'].
     clear H. eapply inversion_Proj in Ht' as (?&?&?&?&?&?&?&?&?&?); auto.
     eapply elim_restriction_works_proj; eauto. exact d.
     intros isp. eapply isErasable_Proof in isp; eauto.
+
+  - cbn.
+    pose proof Hmfix as Hmfix'.
+    specialize (Hmfix' Σ eq_refl). destruct Hmfix'.
+    depelim X0. destruct a.
+    assert (exists na ty bod, dbody d = tLambda na ty bod).
+    { clear -H0. destruct (dbody d) => //. now do 3 eexists. }
+    destruct H2 as [na [ty [bod eq]]]. rewrite {1 3}eq /= //.
+    move: H. rewrite {1}eq.
+    set (et := erase _ _ _ _). clearbody et.
+    intros He. depelim He. cbn.
+    split => //. cbn. rewrite eq. now constructor.
+    split => //. cbn. rewrite eq.
+    destruct H1.
+    eapply Is_type_lambda in X1; tea. 2:pcuic. destruct X1.
+    now constructor.
 Qed.
 
 Transparent wf_reduction.
@@ -1091,10 +1128,10 @@ Proof.
     eapply Hdef; eauto.
 Qed.
 
-Lemma erase_global_erases_deps {Σ} {Σ' : EAst.global_declarations} {t et T} : 
+Lemma erase_global_erases_deps {Σ} {Σ' : EAst.global_declarations} {Γ t et T} : 
   wf_ext Σ ->
-  Σ;;; [] |- t : T ->
-  Σ;;; [] |- t ⇝ℇ et ->
+  Σ;;; Γ |- t : T ->
+  Σ;;; Γ |- t ⇝ℇ et ->
   includes_deps Σ Σ' (term_global_deps et) ->
   erases_deps Σ Σ' et.
 Proof.
@@ -1351,7 +1388,7 @@ Qed.
 Lemma erase_constant_body_correct' {Σ : wf_env_ext} {cb} {onc : ∥ on_constant_decl (lift_typing typing) Σ cb ∥} {body} :
   EAst.cst_body (fst (erase_constant_body Σ cb onc)) = Some body ->
   ∥ ∑ t T, (Σ ;;; [] |- t : T) * (Σ ;;; [] |- t ⇝ℇ body) *
-      (term_global_deps body = snd (erase_constant_body Σ cb onc)) ∥.
+    (term_global_deps body = snd (erase_constant_body Σ cb onc)) ∥.
 Proof.
   intros. destruct cb as [name [bod|] univs]; simpl. intros.
   simpl in H. noconf H.
@@ -1780,33 +1817,6 @@ Proof.
   intros fr. now eapply erase_global_decls_fresh.
 Qed.
 
-Lemma erase_global_decls_wf_glob Σ deps decls heq :
-  let Σ' := erase_global_decls deps Σ decls heq in
-  wf_glob Σ'.
-Proof.
-  cbn.
-  revert deps Σ heq.
-  induction decls; [cbn; auto|].
-  { intros. constructor. }
-  intros. destruct a as [kn []]; simpl; destruct KernameSet.mem.
-  + constructor. eapply IHdecls => //.
-    eapply erase_global_decls_fresh; auto.
-    destruct Σ.(referenced_impl_wf).
-    destruct X. rewrite heq in o0. now depelim o0.
-  + cbn.
-    eapply IHdecls.
-  + constructor. eapply IHdecls.
-    eapply erase_global_decls_fresh.
-    destruct Σ.(referenced_impl_wf) as [[onu ond]].
-    rewrite heq in ond. now depelim ond.
-  + eapply IHdecls.
-Qed.
-
-Lemma erase_global_wf_glob Σ deps :
-  let Σ' := erase_global deps Σ in
-  wf_glob Σ'.
-Proof. eapply erase_global_decls_wf_glob. Qed.
-
 From MetaCoq.Erasure Require Import EEtaExpandedFix.
 
 Lemma All_map_All {A B C} {Q : C -> Type} {P : C -> A -> Prop}
@@ -1830,13 +1840,33 @@ Proof.
   rewrite -H. eapply erase_irrel.
 Qed.
 
-Lemma erase_mfix_eq Σ Γ ts wt : 
-  erase_mfix Σ Γ ts wt = map_All (fun d wt => 
+Lemma erase_fix_eq Σ Γ ts wt : 
+  erase_fix Σ Γ ts wt = map_All (fun d wt => 
+    let dbody' := erase Σ _ (dbody d) (fun Σ abs => proj2 (wt Σ abs)) in
+    let dbody' := if isBox dbody' then
+        match d.(dbody) with
+        | tLambda na _ _ => E.tLambda (binder_name na) E.tBox
+        | _ => dbody'
+        end else dbody' 
+    in
+    {| E.dname := d.(dname).(binder_name); E.rarg := d.(rarg); E.dbody := dbody' |}) ts wt.
+Proof.
+  funelim (map_All _ ts wt); cbn; auto.
+  f_equal => //. f_equal => //.
+  rewrite (fst (erase_irrel _) _ _ _ (fun (Σ0 : global_env_ext) (abs : Σ0 = Σ) =>
+  (map_All_obligation_1 x xs h Σ0 abs).p2)).
+  destruct erase => //.
+  rewrite -H. eapply erase_irrel.
+Qed.
+
+Lemma erase_cofix_eq Σ Γ ts wt : 
+  erase_cofix Σ Γ ts wt = map_All (fun d wt => 
     let dbody' := erase Σ _ (dbody d) wt in
     {| E.dname := d.(dname).(binder_name); E.rarg := d.(rarg); E.dbody := dbody' |}) ts wt.
 Proof.
   funelim (map_All _ ts wt); cbn; auto.
-  f_equal => //. f_equal => //. apply erase_irrel.
+  f_equal => //. f_equal => //.
+  apply erase_irrel.
   rewrite -H. eapply erase_irrel.
 Qed.
 
@@ -1848,6 +1878,7 @@ Proof.
     (fun Γ t wt e => ~ (PCUICEtaExpand.isConstruct t || PCUICEtaExpand.isFix t || PCUICEtaExpand.isRel t) -> ~ (isConstruct e || isFix e || isRel e))
     (fun Γ l awt e => True)
     (fun Γ p l awt e => True)
+    (fun Γ l awt e => True)
     (fun Γ l awt e => True)); intros => //. bang.
 Qed.
 
@@ -1878,6 +1909,9 @@ Proof.
     + eexists. reflexivity.
     + now eapply H.
 Qed.
+
+Lemma isLambda_inv t : isLambda t -> exists na ty bod, t = tLambda na ty bod.
+Proof. destruct t => //; eauto. Qed.
 
 Lemma eta_expand_erase {Σ : wf_env_ext} Σ' {Γ t} 
   (wt : forall Σ0 : global_env_ext, abstract_env_rel' Σ Σ0 -> welltyped Σ0 Γ t) Γ' :
@@ -1955,22 +1989,33 @@ Proof.
         -- sq. cbn. eapply nth_error_map_All in H4 as [D Hnth].
            eapply expanded_tFix.
            3:{ destruct args; cbn in *; congruence. }
-          { rewrite erase_mfix_eq. solve_all. eapply All_map_All.
-            intros. eapply H0. intros. cbn in H |- *. destruct H.
-            eapply apply_expanded. eapply e1. eauto.
-            2: reflexivity. 2: eauto.
+          { rewrite erase_fix_eq. solve_all. eapply All_map_All.
+            intros. eapply H0. intros. cbn in H |- *. destruct H as [[isl H] H'].
+            2:reflexivity.
+            epose proof (erases_isLambda (@erases_erase Σ (fix_context mfix ++ Γ) (dbody x)
+            (fun (Σ0 : global_env_ext) (abs : Σ0 = Σ) => (rx Σ0 abs).p2)) isl).
+            destruct (isLambda_inv _ isl) as [na [ty [bod eq]]].
+            split.
+            rewrite {4}eq.
+            destruct isBox eqn:isb => //.
+            set (et := erase _ _ _ _) in *.
+            now rewrite orb_false_r in H1.
+            set (et := erase _ _ _ _) in *.
+            destruct isBox. rewrite eq. constructor. constructor.
+            eapply apply_expanded. eapply H'. eauto.
+            2:{ reflexivity. }
             rewrite !rev_map_spec. do 2 f_equal. clear. 
             generalize (erase_obligation_13 Σ Γ mfix idx Hyp0).
             generalize (fix_context mfix). generalize mfix. clear.
             intros. induction mfix; cbn; f_equal. eapply IHmfix.
           }
            { solve_all.  clear - deps H2. induction H2; econstructor; eauto. eapply p. eauto. }
-           { rewrite erase_mfix_eq. eapply Hnth. }
+           { rewrite erase_fix_eq. eapply Hnth. }
            rewrite map_erase_length. cbn. lia.
       * eapply typing_wf_local; eauto.
       * cbn; intros; subst. eapply welltyped_mkApps_inv; sq; eauto. 
   - econstructor; eauto.
-    solve_all. rewrite erase_mfix_eq.
+    solve_all. rewrite erase_cofix_eq.
     eapply All_map_All. intros. exact H0. intros x y wx [exp' IH]. len. eauto. eauto.
   - simp erase. destruct inspect as [b ise] eqn:hi. destruct b.
     + simp erase. constructor.
@@ -2044,23 +2089,221 @@ Proof.
 Qed.
 
 Lemma erases_deps_erase (cf := config.extraction_checker_flags) {Σ : wf_env} univs (wfΣ : ∥ wf_ext (Σ, univs) ∥)
-  (Σ' := make_wf_env_ext Σ univs wfΣ) t 
-  (wt : forall Σ0 : global_env_ext, abstract_env_rel' Σ' Σ0 -> PCUICSafeLemmata.welltyped Σ0 [] t) :
-  let et := erase Σ' [] t wt in
+  (Σ' := make_wf_env_ext Σ univs wfΣ) Γ t 
+  (wt : forall Σ0 : global_env_ext, abstract_env_rel' Σ' Σ0 -> PCUICSafeLemmata.welltyped Σ0 Γ t) :
+  let et := erase Σ' Γ t wt in
   let deps := EAstUtils.term_global_deps et in
   erases_deps Σ (erase_global deps Σ) et.
 Proof.
   intros et deps. destruct wfΣ.
   pose proof (wt Σ' eq_refl). destruct H.
   eapply (erase_global_erases_deps w); tea.
-  eapply (erases_erase (Σ := Σ') (Γ := [])).
+  eapply (erases_erase (Σ := Σ') (Γ := Γ)).
   eapply erase_global_includes.
   intros.
   eapply term_global_deps_spec in H; eauto.
   assumption.
-  eapply (erases_erase (Σ := Σ') (Γ := [])).
+  eapply (erases_erase (Σ := Σ') (Γ := Γ)).
   eapply KernameSet.subset_spec. reflexivity. 
 Qed.
+
+Lemma erases_deps_erase_weaken (cf := config.extraction_checker_flags) {Σ : wf_env} univs
+  (wfΣ : ∥ wf_ext (Σ, univs) ∥) Γ
+  (Σ' := make_wf_env_ext Σ univs wfΣ) t 
+  (wt : forall Σ0 : global_env_ext, abstract_env_rel' Σ' Σ0 -> PCUICSafeLemmata.welltyped Σ0 Γ t) 
+  deps :
+  let et := erase Σ' Γ t wt in
+  let tdeps := EAstUtils.term_global_deps et in
+  erases_deps Σ (erase_global (KernameSet.union deps tdeps) Σ) et.
+Proof.
+  intros et tdeps. destruct wfΣ.
+  pose proof (wt Σ' eq_refl). destruct H.
+  eapply (erase_global_erases_deps w); tea.
+  eapply (erases_erase (Σ := Σ') (Γ := Γ)).
+  eapply erase_global_includes.
+  intros.
+  eapply term_global_deps_spec in H; eauto.
+  assumption.
+  eapply (erases_erase (Σ := Σ') (Γ := Γ)).
+  eapply KernameSet.subset_spec. intros x hin. eapply KernameSet.union_spec. now right.
+Qed.
+
+Import EWellformed.
+
+Section wffix.
+  Import EAst.
+  Fixpoint wf_fixpoints (t : term) : bool :=
+    match t with
+    | tRel i => true
+    | tEvar ev args => List.forallb (wf_fixpoints) args
+    | tLambda N M => wf_fixpoints M
+    | tApp u v => wf_fixpoints u && wf_fixpoints v
+    | tLetIn na b b' => wf_fixpoints b && wf_fixpoints b'
+    | tCase ind c brs => 
+      let brs' := forallb (wf_fixpoints ∘ snd) brs in
+      wf_fixpoints c && brs'
+    | tProj p c => wf_fixpoints c
+    | tFix mfix idx => 
+      List.forallb (fun d => (isLambda d.(dbody) || isBox d.(dbody)) && wf_fixpoints d.(dbody)) mfix
+    | tCoFix mfix idx =>
+      List.forallb (wf_fixpoints ∘ dbody) mfix
+    | tConst kn => true
+    | tConstruct ind c => true
+    | tVar _ => true
+    | tBox => true
+    end.
+
+End wffix.
+
+
+Lemma erases_deps_wellformed (cf := config.extraction_checker_flags) (efl := all_env_flags) {Σ} {Σ'} et :
+  erases_deps Σ Σ' et ->
+  forall n, ELiftSubst.closedn n et ->
+  wf_fixpoints et ->
+  wellformed Σ' n et.
+Proof.
+  intros ed.
+  induction ed using erases_deps_forall_ind; intros => //; 
+   try solve [cbn in *; rtoProp; intuition eauto; solve_all].
+  - cbn. red in H0. rewrite H0 //.
+  - cbn -[lookup_constructor].
+    cbn. now destruct H0 as [[-> ->] ->].
+  - cbn in *. move/andP: H5 => [] cld clbrs.
+    cbn. apply/andP; split. apply/andP; split. 
+    * now destruct H0 as [-> ->].
+    * now move/andP: H6.
+    * move/andP: H6; solve_all.
+  - cbn in *. apply/andP; split; eauto.
+    now destruct H0 as [-> ->].
+Qed.
+
+Lemma erases_wf_fixpoints Σ Γ t t' : Σ;;; Γ |- t ⇝ℇ t' -> 
+  ErasureCorrectness.wellformed Σ t -> wf_fixpoints t'.
+Proof.
+  induction 1 using erases_forall_list_ind; cbn; auto; try solve [rtoProp; repeat solve_all].
+  - unfold test_def in *.
+    eapply Forall2_All2 in H.
+    eapply All2_All2_mix in X; tea. solve_all.
+    destruct b0; eapply erases_isLambda in H1; tea.
+  - unfold test_def in *. solve_all.
+Qed.
+
+Lemma erase_wf_fixpoints (efl := all_env_flags) {Σ : wf_env} univs wfΣ {Γ t} wt
+  (Σ' := make_wf_env_ext Σ univs wfΣ) :
+  let t' := erase Σ' Γ t wt in
+  wf_fixpoints t'.
+Proof.
+  cbn.
+  eapply erases_wf_fixpoints.
+  eapply erases_erase.
+  specialize (wt (Σ, univs) eq_refl).
+  destruct wfΣ.
+  now unshelve eapply welltyped_wellformed in wt. 
+Qed.
+
+Lemma erase_wellformed (efl := all_env_flags) {Σ : wf_env} univs wfΣ {Γ t} wt
+  (Σ' := make_wf_env_ext Σ univs wfΣ) :
+  let t' := erase Σ' Γ t wt in
+  wellformed (erase_global (term_global_deps t') Σ) #|Γ| t'.
+Proof.
+  set (t' := erase _ _ _ _).
+  cbn.
+  epose proof (@erases_deps_erase Σ univs wfΣ Γ t wt).
+  cbn in H.
+  epose proof (erases_deps_wellformed _ H #|Γ|).
+  apply H0.
+  eapply (erases_closed _ Γ). eapply erases_erase.
+  destruct (wt _ eq_refl).
+  cbn in X. destruct wfΣ.
+  now eapply PCUICClosedTyp.subject_closed in X.
+  eapply erase_wf_fixpoints.
+Qed.
+
+Lemma erase_wellformed_weaken (efl := all_env_flags) {Σ : wf_env} univs wfΣ {Γ t} wt deps
+  (Σ' := make_wf_env_ext Σ univs wfΣ) :
+  let t' := erase Σ' Γ t wt in
+  wellformed (erase_global (KernameSet.union deps (term_global_deps t')) Σ) #|Γ| t'.
+Proof.
+  set (t' := erase _ _ _ _).
+  cbn.
+  epose proof (@erases_deps_erase_weaken Σ univs wfΣ Γ t wt deps).
+  cbn in H.
+  epose proof (erases_deps_wellformed _ H #|Γ|).
+  apply H0.
+  eapply (erases_closed _ Γ). eapply erases_erase.
+  destruct (wt _ eq_refl).
+  cbn in X. destruct wfΣ.
+  now eapply PCUICClosedTyp.subject_closed in X.
+  eapply erase_wf_fixpoints.
+Qed.
+
+Lemma erase_constant_body_correct'' {Σ : wf_env} {cb} {univs wfΣ}
+(Σ' := make_wf_env_ext Σ univs wfΣ)
+{onc : ∥ on_constant_decl (lift_typing typing) Σ' cb ∥} {body} deps :  
+  EAst.cst_body (fst (erase_constant_body Σ' cb onc)) = Some body ->
+  ∥ ∑ t T, (Σ' ;;; [] |- t : T) * (Σ' ;;; [] |- t ⇝ℇ body) *
+      (term_global_deps body = snd (erase_constant_body Σ' cb onc)) *
+      wellformed (sw:=all_env_flags) (erase_global (KernameSet.union deps (term_global_deps body)) Σ) 0 body ∥.
+Proof.
+  intros. destruct cb as [name [bod|] udecl]; simpl. intros.
+  simpl in H. noconf H.
+  set (obl :=(erase_constant_body_obligation_1 Σ'
+  {|
+  cst_type := name;
+  cst_body := Some bod;
+  cst_universes := udecl |} onc bod eq_refl)). clearbody obl.
+  assert (wfΣ' : abstract_env_rel' Σ' Σ') by reflexivity.
+  destruct (obl _ wfΣ'). sq.
+  have er : (Σ, univs);;; [] |- bod ⇝ℇ erase (make_wf_env_ext Σ univs (sq w)) [] bod obl.
+  { eapply (erases_erase (Σ:=Σ')). }
+  exists bod, A; intuition auto. eapply erase_wellformed_weaken.
+  now simpl in H.
+Qed.
+
+Lemma erase_global_decl_wf_glob Σ deps decls heq :
+  forall cb wfΣ hcb,
+  let ecb := erase_constant_body (make_wf_env_ext Σ (cst_universes cb) wfΣ) cb hcb in
+  let Σ' := erase_global_decls (KernameSet.union deps ecb.2) Σ decls heq in
+  @wf_global_decl all_env_flags Σ' (EAst.ConstantDecl ecb.1).
+Proof.
+  intros cb wfΣ hcb.
+  set (ecb := erase_constant_body _ _ _). cbn.
+  unfold wf_global_decl. cbn.
+  destruct wfΣ, hcb. red in o.
+  destruct EAst.cst_body eqn:hb => /= //. subst decls.
+  eapply (erase_constant_body_correct'') in hb.
+  destruct hb. destruct X as [t0 [T [[] ?]]].
+  set(Σext := make_wf_env_ext _ _ _) in *.
+  destruct p. rewrite e in i. exact i.  
+Qed.
+
+Lemma erase_global_decls_wf_glob Σ deps decls heq :
+  let Σ' := erase_global_decls deps Σ decls heq in
+  @wf_glob all_env_flags Σ'.
+Proof.
+  cbn.
+  revert deps Σ heq.
+  induction decls; [cbn; auto|].
+  { intros. constructor. }
+  intros. destruct a as [kn []]; simpl; destruct KernameSet.mem.
+  + constructor. eapply IHdecls => //. eapply erase_global_decl_wf_glob; auto.
+    eapply erase_global_decls_fresh; auto.
+    destruct Σ.(referenced_impl_wf).
+    destruct X. rewrite heq in o0. now depelim o0.
+  + cbn.
+    eapply IHdecls.
+  + constructor. eapply IHdecls. constructor.
+    eapply erase_global_decls_fresh.
+    destruct Σ.(referenced_impl_wf) as [[onu ond]].
+    rewrite heq in ond. now depelim ond.
+  + eapply IHdecls.
+Qed.
+
+Lemma erase_global_wf_glob Σ deps :
+  let Σ' := erase_global deps Σ in
+  @wf_glob all_env_flags Σ'.
+Proof. eapply erase_global_decls_wf_glob. Qed.
+
 
 Lemma lookup_erase_global (cf := config.extraction_checker_flags) {Σ : wf_env} {deps deps'} :
   KernameSet.Subset deps deps' ->
@@ -2086,10 +2329,11 @@ Proof.
     + destruct (KernameSet.mem kn' deps') eqn:eq'.
       eapply EExtends.global_subset_cons_right.
       eapply erase_global_wf_glob.
+      unfold decl. unfold hidebody.
       constructor. eapply erase_global_wf_glob.
-      eapply erase_global_decls_fresh.
-      clear -wfΣ. destruct wfΣ. destruct X as [onu ond]; cbn in *.
-      now depelim ond.
+      eapply erase_global_decl_wf_glob.
+      depelim wfΣ. depelim w. cbn in o0. depelim o0.
+      eapply erase_global_decls_fresh => //.
       eapply IHΣ.
       intros x hin.
       eapply KernameSet.union_spec. left. now eapply sub.
@@ -2099,8 +2343,8 @@ Proof.
       apply EExtends.global_subset_cons. eapply IHΣ => //.
     + destruct (KernameSet.mem kn' deps') eqn:eq'.
       eapply EExtends.global_subset_cons_right. eapply erase_global_wf_glob.
-      constructor. eapply erase_global_wf_glob.
-      eapply erase_global_decls_fresh.
+      constructor. eapply erase_global_wf_glob. constructor.
+      eapply erase_global_decls_fresh => //.
       clear -wfΣ. destruct wfΣ. destruct X as [onu ond]; cbn in *. now depelim ond.
       eapply IHΣ. intros x hin. now eapply sub.
       eapply IHΣ => //. }
@@ -2113,11 +2357,12 @@ Lemma expanded_weakening_global Σ deps deps' Γ t :
 Proof.
   intros hs.
   eapply expanded_ind; intros; try solve [econstructor; eauto].
-  eapply expanded_tConstruct_app; tea.
-  destruct H. split; tea.
-  destruct d; split => //.
-  cbn in *. red in H.
-  eapply lookup_erase_global in H; tea.
+  - eapply expanded_tFix; tea. solve_all.
+  - eapply expanded_tConstruct_app; tea.
+    destruct H. split; tea.
+    destruct d; split => //.
+    cbn in *. red in H.
+    eapply lookup_erase_global in H; tea.
 Qed.
 
 Lemma expanded_erase (cf := config.extraction_checker_flags) {Σ : wf_env} univs wfΣ t wtp :
