erasure/theories/ETransform.v
@@ -7,11 +7,11 @@ Set Warnings "-notation-overridden".
 From MetaCoq.PCUIC Require PCUICAst PCUICAstUtils PCUICProgram PCUICTransform.
 Set Warnings "+notation-overridden".
 From MetaCoq.SafeChecker Require Import PCUICErrors PCUICWfEnvImpl.
-From MetaCoq.Erasure Require EAstUtils ErasureFunction ErasureCorrectness EPretty Extract EProgram.
+From MetaCoq.Erasure Require EAstUtils ErasureFunction ErasureCorrectness EPretty Extract EOptimizePropDiscr ERemoveParams EProgram.
 
 Import PCUICAst (term) PCUICProgram PCUICTransform (eval_pcuic_program) Extract EProgram
-    EAst Transform.
-Import EEnvMap EGlobalEnv.
+    EAst Transform ERemoveParams.
+Import EEnvMap EGlobalEnv EWellformed.
 
 Program Definition erase_transform : Transform.t pcuic_program eprogram_env PCUICAst.term EAst.term 
   eval_pcuic_program (eval_eprogram_env EWcbvEval.default_wcbv_flags) :=
@@ -19,24 +19,16 @@ Program Definition erase_transform : Transform.t pcuic_program eprogram_env PCUI
     pre p :=  
       ∥ wt_pcuic_program (cf := config.extraction_checker_flags) p ∥ /\ PCUICEtaExpand.expanded_pcuic_program p ;
     transform p hp := erase_program p (proj1 hp) ;
-    post p :=
-      let decls := p.1.(GlobalContextMap.global_decls) in
-      [/\ wf_glob decls, closed_eprogram_env p & expanded_eprogram p];
+    post p := [/\ wf_eprogram_env all_env_flags p & expanded_eprogram_env p];
     obseq g g' v v' := let Σ := g.1 in Σ ;;; [] |- v ⇝ℇ v' |}.
 Next Obligation.
   cbn -[erase_program].
   intros p [wtp etap].
   destruct erase_program eqn:e.
   split; cbn.
-  - unfold erase_program, erase_pcuic_program in e. simpl. injection e. intros <- <-. 
-    eapply ErasureFunction.erase_global_wf_glob.
-  - apply/andP; split.
-    * unfold erase_program, erase_pcuic_program in e. simpl. injection e. intros <- <-. 
-      eapply ErasureFunction.erase_global_closed.
-    * unfold erase_program, erase_pcuic_program in e. simpl. injection e. intros <- <-. 
-      eapply (ErasureFunction.erases_closed _ []). eapply ErasureFunction.erases_erase.
-      clear e. destruct wtp as [[wfΣ [T HT]]].
-      now eapply (@PCUICClosedTyp.subject_closed _ _) in HT.
+  - unfold erase_program, erase_pcuic_program in e. simpl. injection e. intros <- <-.
+    split. 
+    eapply ErasureFunction.erase_global_wf_glob. eapply ErasureFunction.erase_wellformed.
   - rewrite -e. cbn.
     now eapply expanded_erase_program.
 Qed.
@@ -61,114 +53,99 @@ Qed.
 
 Import EWcbvEval (WcbvFlags, with_prop_case, with_guarded_fix).
 
-Program Definition guarded_to_unguarded_fix {fl : EWcbvEval.WcbvFlags} (wguard : with_guarded_fix) :
+Program Definition guarded_to_unguarded_fix {fl : EWcbvEval.WcbvFlags} {efl : EEnvFlags} (wguard : with_guarded_fix) :
   Transform.t eprogram_env eprogram_env EAst.term EAst.term 
     (eval_eprogram_env fl) (eval_eprogram_env (EEtaExpandedFix.switch_unguarded_fix fl)) :=
   {| name := "switching to unguarded fixpoints";
     transform p pre := p;
-    pre p := 
-    let decls := p.1.(GlobalContextMap.global_decls) in
-     [/\ wf_glob decls, closed_eprogram_env p & expanded_eprogram p ];
-    post p := let decls := p.1.(GlobalContextMap.global_decls) in
-     [/\ wf_glob decls, closed_eprogram_env p & expanded_eprogram p ];
+    pre p := wf_eprogram_env efl p /\ expanded_eprogram_env p;
+    post p := wf_eprogram_env efl p /\ expanded_eprogram_env p;
     obseq g g' v v' := v' = v |}.
 Next Obligation. cbn. eauto. Qed.
 Next Obligation.
   cbn.
-  move=> fl wguard [Σ t] v [wfe /andP[cle clt] /andP[etae etat]]. cbn in *.
+  move=> fl efl wguard [Σ t] v [wfp /andP[etae etat]]. cbn in *.
   intros [ev]. exists v. split => //.
   red. sq. cbn in *.
-  now apply EEtaExpandedFix.eval_opt_to_target.
+  apply EEtaExpandedFix.eval_opt_to_target => //. apply wfp.
 Qed.
 
-Program Definition remove_params (p : eprogram_env) : eprogram :=
-  (ERemoveParams.strip_env p.1, ERemoveParams.strip p.1 p.2).
-
-Program Definition remove_params_optimization {fl : EWcbvEval.WcbvFlags} : 
+Program Definition remove_params_optimization {fl : EWcbvEval.WcbvFlags} 
+  (efl := all_env_flags): 
   Transform.t eprogram_env eprogram EAst.term EAst.term (eval_eprogram_env fl) (eval_eprogram fl) :=
   {| name := "stripping constructor parameters";
-    transform p pre := remove_params p;
-    pre p := 
-    let decls := p.1.(GlobalContextMap.global_decls) in
-     [/\ wf_glob decls, closed_eprogram_env p & expanded_eprogram_cstrs p ];
-    post := closed_eprogram;
+    transform p pre := ERemoveParams.strip_program p;
+    pre p := wf_eprogram_env efl p /\ expanded_eprogram_env_cstrs p;
+    post p := wf_eprogram (switch_no_params efl) p /\ expanded_eprogram_cstrs p;
     obseq g g' v v' := v' = (ERemoveParams.strip g.1 v) |}.
 Next Obligation.
-  move=> fl [Σ t] [wfe /andP[cle clt] etap].
+  move=> fl efl [Σ t] [wfp etap].
   simpl.
   cbn -[ERemoveParams.strip] in *.
-  apply/andP; split; cbn.
-  move: cle. unfold closed_env. unfold ERemoveParams.strip_env.
-  rewrite forallb_map. eapply forallb_impl. intros.
-  destruct x as [kn []]; cbn in * => //.
-  destruct Extract.E.cst_body => //. cbn -[ERemoveParams.strip] in H0 |- *.
-  now eapply ERemoveParams.closed_strip.
-  now eapply ERemoveParams.closed_strip.
+  split. now eapply ERemoveParams.strip_program_wf.
+  now eapply ERemoveParams.strip_program_expanded.
 Qed.
 
 Next Obligation.
-  red. move=> ? [Σ t] /= v [wfe /andP[cle clt] etap] [ev].
+  red. move=> ? [Σ t] /= v [[wfe wft] etap] [ev].
   eapply ERemoveParams.strip_eval in ev; eauto.
-  eexists; split => //. now sq.
-  all:move/andP: etap => [] => //.
+  eexists; split => /= //. now sq. cbn in *.
+  now eapply wellformed_closed_env.
+  now move/andP: etap.
+  now eapply wellformed_closed.
+  now move/andP: etap.
 Qed.
 
-Program Definition remove_params_fast_optimization (fl : EWcbvEval.WcbvFlags) :
+Program Definition remove_params_fast_optimization (fl : EWcbvEval.WcbvFlags)
+  (efl := all_env_flags) :
   Transform.t eprogram_env eprogram EAst.term EAst.term (eval_eprogram_env fl) (eval_eprogram fl) :=
   {| name := "stripping constructor parameters (faster?)";
     transform p _ := (ERemoveParams.Fast.strip_env p.1, ERemoveParams.Fast.strip p.1 [] p.2);
-    pre p := 
-      let decls := p.1.(GlobalContextMap.global_decls) in
-      [/\ wf_glob decls, closed_eprogram_env p & expanded_eprogram_cstrs p];
-    post := closed_eprogram;
+    pre p := wf_eprogram_env efl p /\ expanded_eprogram_env_cstrs p;
+    post p := wf_eprogram (switch_no_params efl) p /\ expanded_eprogram_cstrs p;
     obseq g g' v v' := v' = (ERemoveParams.strip g.1 v) |}.
 Next Obligation.
-  move=> fl [Σ t] [wfe /andP[cle clt] etap].
+  move=> fl efl [Σ t] [wfp etap].
   simpl.
-  apply/andP.
-  rewrite -ERemoveParams.Fast.strip_fast -ERemoveParams.Fast.strip_env_fast.
   cbn -[ERemoveParams.strip] in *.
-  split.
-  move: cle. unfold closed_env. unfold ERemoveParams.strip_env.
-  rewrite forallb_map. eapply forallb_impl. intros.
-  destruct x as [kn []]; cbn in * => //.
-  destruct Extract.E.cst_body => //. cbn -[ERemoveParams.strip] in H0 |- *.
-  now eapply ERemoveParams.closed_strip.
-  now eapply ERemoveParams.closed_strip.
+  rewrite -ERemoveParams.Fast.strip_fast -ERemoveParams.Fast.strip_env_fast.
+  split. 
+  now eapply (ERemoveParams.strip_program_wf (Σ, t)).
+  now eapply (ERemoveParams.strip_program_expanded (Σ, t)).
 Qed.
+
 Next Obligation.
-  red. move=> ? [Σ t] /= v [wfe /andP[cle clt] etap] [ev].
+  red. move=> ? [Σ t] /= v [[wfe wft] etap] [ev].
   rewrite -ERemoveParams.Fast.strip_fast -ERemoveParams.Fast.strip_env_fast.
   eapply ERemoveParams.strip_eval in ev; eauto.
-  eexists; split => //. now sq.
-  all:move/andP: etap => [] => //.
+  eexists; split => /= //.
+  now sq. cbn in *.
+  now eapply wellformed_closed_env.
+  now move/andP: etap.
+  now eapply wellformed_closed.
+  now move/andP: etap.
 Qed.
 
 Import EOptimizePropDiscr EWcbvEval.
 
-Program Definition optimize_prop_discr_optimization {fl : WcbvFlags} : 
-  self_transform eprogram EAst.term (eval_eprogram fl) 
-    (eval_eprogram (disable_prop_cases fl)) := 
+Program Definition optimize_prop_discr_optimization {fl : WcbvFlags} {efl : EEnvFlags} {hastrel : has_tRel} {hastbox : has_tBox} :
+  self_transform eprogram EAst.term (eval_eprogram fl) (eval_eprogram (disable_prop_cases fl)) := 
   {| name := "optimize_prop_discr"; 
-    transform p _ := 
-      (EOptimizePropDiscr.optimize_env p.1, EOptimizePropDiscr.optimize p.1 p.2);
-    pre := closed_eprogram;
-    post := closed_eprogram;
-    obseq g g' v v' := v' = EOptimizePropDiscr.optimize g.1 v
-    |}.
+    transform p _ := optimize_program p ; 
+    pre p := wf_eprogram efl p /\ expanded_eprogram_cstrs p;
+    post p := wf_eprogram efl p /\ expanded_eprogram_cstrs p;
+    obseq g g' v v' := v' = EOptimizePropDiscr.optimize g.1 v |}.
 
 Next Obligation.
-  move=> fl [Σ t] /andP[cle clt].
-  cbn in *. apply/andP; split.
-  move: cle. cbn. induction Σ at 1 3; cbn; auto.
-  move/andP => [] cla clg. rewrite (IHg clg) andb_true_r.
-  destruct a as [kn []]; cbn in * => //.
-  destruct Extract.E.cst_body => //. cbn in cla |- *.
-  now eapply EOptimizePropDiscr.closed_optimize.
-  now eapply EOptimizePropDiscr.closed_optimize.
+  move=> fl efl hastrel hastbox [Σ t] [wfp etap].
+  cbn in *. split.
+  - now eapply optimize_program_wf.
+  - now eapply optimize_program_expanded.
 Qed.
 Next Obligation.
-  red. move=> fl [Σ t] /= v /andP[cle clt] [ev].
+  red. move=> fl efl hastrel hastbox [Σ t] /= v [wfe wft] [ev].
   eapply EOptimizePropDiscr.optimize_correct in ev; eauto.
-  eexists; split => //. red. sq; auto.
+  eexists; split => //. red. sq; auto. cbn. apply wfe.
+  eapply wellformed_closed_env, wfe.
+  eapply wellformed_closed, wfe.
 Qed.
